src/Init/Data/Vector/Basic.lean
@@ -180,7 +180,7 @@ which also receives the index of the element, and the fact that the index is les
   ⟨v.toArray.mapFinIdx (fun i a h => f i a (by simpa [v.size_toArray] using h)), by simp⟩
 
 /-- Map a monadic function over a vector. -/
-def mapM [Monad m] (f : α → m β) (v : Vector α n) : m (Vector β n) := do
+@[inline] def mapM [Monad m] (f : α → m β) (v : Vector α n) : m (Vector β n) := do
   go 0 (Nat.zero_le n) #v[]
 where
   go (i : Nat) (h : i ≤ n) (r : Vector β i) : m (Vector β n) := do
@@ -188,6 +188,40 @@ where
       go (i+1) (by omega) (r.push (← f v[i]))
     else
       return r.cast (by omega)
+
+@[inline] def forM [Monad m] (v : Vector α n) (f : α → m PUnit) : m PUnit :=
+  v.toArray.forM f
+
+@[inline] def flatMapM [Monad m] (v : Vector α n) (f : α → m (Vector β k)) : m (Vector β (n * k)) := do
+  go 0 (Nat.zero_le n) (#v[].cast (by omega))
+where
+  go (i : Nat) (h : i ≤ n) (r : Vector β (i * k)) : m (Vector β (n * k)) := do
+    if h' : i < n then
+      go (i+1) (by omega) ((r ++ (← f v[i])).cast (Nat.succ_mul i k).symm)
+    else
+      return r.cast (by congr; omega)
+
+/-- Variant of `mapIdxM` which receives the index `i` along with the bound `i < n. -/
+@[inline]
+def mapFinIdxM {α : Type u} {β : Type v} {m : Type v → Type w} [Monad m]
+    (as : Vector α n) (f : (i : Nat) → α → (h : i < n) → m β) : m (Vector β n) :=
+  let rec @[specialize] map (i : Nat) (j : Nat) (inv : i + j = n) (bs : Vector β (n - i)) : m (Vector β n) := do
+    match i, inv with
+    | 0,    _  => pure bs
+    | i+1, inv =>
+      have j_lt : j < n := by
+        rw [← inv, Nat.add_assoc, Nat.add_comm 1 j, Nat.add_comm]
+        apply Nat.le_add_right
+      have : i + (j + 1) = n := by rw [← inv, Nat.add_comm j 1, Nat.add_assoc]
+      map i (j+1) this ((bs.push (← f j as[j] j_lt)).cast (by omega))
+  map n 0 rfl (#v[].cast (by simp))
+
+@[inline]
+def mapIdxM {α : Type u} {β : Type v} {m : Type v → Type w} [Monad m] (f : Nat → α → m β) (as : Vector α n) : m (Vector β n) :=
+  as.mapFinIdxM fun i a _ => f i a
+
+@[inline] def firstM {α : Type u} {m : Type v → Type w} [Alternative m] (f : α → m β) (as : Vector α n) : m β :=
+  as.toArray.firstM f
 
 @[inline] def flatten (v : Vector (Vector α n) m) : Vector α (m * n) :=
   ⟨(v.toArray.map Vector.toArray).flatten,
@@ -312,6 +346,16 @@ no element of the index matches the given value.
 @[inline] def indexOf? [BEq α] (v : Vector α n) (x : α) : Option (Fin n) :=
   (v.toArray.indexOf? x).map (Fin.cast v.size_toArray)
 
+/--
+Note that the universe level is contrained to `Type` here,
+to avoid having to have the predicate live in `p : α → m (ULift Bool)`.
+-/
+@[inline] def findM? {α : Type} {m : Type → Type} [Monad m] (f : α → m Bool) (as : Vector α n) : m (Option α) :=
+  as.toArray.findM? f
+
+@[inline] def findSomeM? [Monad m] (f : α → m (Option β)) (as : Vector α n) : m (Option β) :=
+  as.toArray.findSomeM? f
+
 /-- Returns `true` when `v` is a prefix of the vector `w`. -/
 @[inline] def isPrefixOf [BEq α] (v : Vector α m) (w : Vector α n) : Bool :=
   v.toArray.isPrefixOf w.toArray
@@ -348,6 +392,10 @@ no element of the index matches the given value.
 instance : ForIn' m (Vector α n) α inferInstance where
   forIn' v b f := Array.forIn' v.toArray b (fun a h b => f a (by simpa using h) b)
 
+/-! ### ForM instance -/
+
+instance : ForM m (Vector α n) α where
+  forM := forM
 /-! ### ToStream instance -/
 
 instance : ToStream (Vector α n) (Subarray α) where
